extraction/theories/LiftSubst.v
@@ -1,7 +1,9 @@
 (* Distributed under the terms of the MIT license.   *)
 
-From Coq Require Import List Program BinPos Arith.Compare_dec Bool.
+From Coq Require Import List Program BinPos Arith.Compare_dec Bool Lia.
+From Template Require Import Ast AstUtils utils.
 From TemplateExtraction Require Import Ast Induction.
+
 
 (** * Lifting and substitution for the AST
 
@@ -16,8 +18,7 @@ Fixpoint lift n k t : term :=
   | tRel i => if Nat.leb k i then tRel (n + i) else tRel i
   | tEvar ev args => tEvar ev (List.map (lift n k) args)
   | tLambda na T M => tLambda na (lift n k T) (lift n (S k) M)
-  | tApp u v => tApp (lift n k u) (List.map (lift n k) v)
-  | tProd na A B => tProd na (lift n k A) (lift n (S k) B)
+  | tApp u v => tApp (lift n k u) (lift n k v)
   | tLetIn na b t b' => tLetIn na (lift n k b) (lift n k t) (lift n (S k) b')
   | tCase ind p c brs =>
     let brs' := List.map (on_snd (lift n k)) brs in
@@ -25,60 +26,66 @@ Fixpoint lift n k t : term :=
   | tProj p c => tProj p (lift n k c)
   | tFix mfix idx =>
     let k' := List.length mfix + k in
-    let mfix' := List.map (map_def (lift n k')) mfix in
+    let mfix' := List.map (map_def (lift n k) (lift n k')) mfix in
     tFix mfix' idx
   | tCoFix mfix idx =>
     let k' := List.length mfix + k in
-    let mfix' := List.map (map_def (lift n k')) mfix in
+    let mfix' := List.map (map_def (lift n k) (lift n k')) mfix in
     tCoFix mfix' idx
-  | _ => t
+  | tBox => t
+  | tVar _ => t
+  | tMeta _ => t
+  | tConst _ _ => t
+  | tConstruct _ _ _ => t
   end.
 
 
 Notation lift0 n := (lift n 0).
 Definition up := lift 1 0.
 
-Fixpoint subst t k u :=
+(** Parallel substitution: it assumes that all terms in the substitution live in the
+    same context *)
+
+Fixpoint subst s k u :=
   match u with
   | tRel n =>
-    match Nat.compare k n with
-    | Datatypes.Eq => lift0 k t
-    | Datatypes.Gt => tRel n
-    | Datatypes.Lt => tRel (pred n)
-    end
-  | tEvar ev args => tEvar ev (List.map (subst t k) args)
-  | tLambda na T M => tLambda na (subst t k T) (subst t (S k) M)
-  | tApp u v => mkApps (subst t k u) (List.map (subst t k) v)
-  | tProd na A B => tProd na (subst t k A) (subst t (S k) B)
-  | tLetIn na b ty b' => tLetIn na (subst t k b) (subst t k ty) (subst t (S k) b')
+    if Nat.leb k n then
+      match nth_error s (n - k) with
+      | Some b => lift0 k b
+      | None => tRel (n - List.length s)
+      end
+    else tRel n
+  | tEvar ev args => tEvar ev (List.map (subst s k) args)
+  | tLambda na T M => tLambda na (subst s k T) (subst s (S k) M)
+  | tApp u v => tApp (subst s k u) (subst s k v)
+  | tLetIn na b ty b' => tLetIn na (subst s k b) (subst s k ty) (subst s (S k) b')
   | tCase ind p c brs =>
-    let brs' := List.map (on_snd (subst t k)) brs in
-    tCase ind (subst t k p) (subst t k c) brs'
-  | tProj p c => tProj p (subst t k c)
+    let brs' := List.map (on_snd (subst s k)) brs in
+    tCase ind (subst s k p) (subst s k c) brs'
+  | tProj p c => tProj p (subst s k c)
   | tFix mfix idx =>
     let k' := List.length mfix + k in
-    let mfix' := List.map (map_def (subst t k')) mfix in
+    let mfix' := List.map (map_def (subst s k) (subst s k')) mfix in
     tFix mfix' idx
   | tCoFix mfix idx =>
     let k' := List.length mfix + k in
-    let mfix' := List.map (map_def (subst t k')) mfix in
+    let mfix' := List.map (map_def (subst s k) (subst s k')) mfix in
     tCoFix mfix' idx
   | x => x
   end.
 
+(** Substitutes [t1 ; .. ; tn] in u for [Rel 0; .. Rel (n-1)] *in parallel* *)
 Notation subst0 t := (subst t 0).
-Notation "M { j := N }" := (subst N j M) (at level 10, right associativity).
-
-(** Substitutes [t1 ; .. ; tn] in u for [Rel 0; .. Rel (n-1)]*)
-Definition substl l t :=
-  List.fold_left (fun t u => subst0 u t) l t.
+Definition subst1 t k u := subst [t] k u.
+Notation subst10 t := (subst1 t 0).
+Notation "M { j := N }" := (subst1 N j M) (at level 10, right associativity).
 
 Fixpoint closedn k (t : term) : bool :=
   match t with
   | tRel i => Nat.ltb i k
   | tEvar ev args => List.forallb (closedn k) args
-  | tLambda _ T M | tProd _ T M => closedn k T && closedn (S k) M
-  | tApp u v => closedn k u && List.forallb (closedn k) v
+  | tLambda _ T M => closedn k T && closedn (S k) M
+  | tApp u v => closedn k u && closedn k v
   | tLetIn na b t b' => closedn k b && closedn k t && closedn (S k) b'
   | tCase ind p c brs =>
     let brs' := List.forallb (test_snd (closedn k)) brs in
@@ -86,10 +93,10 @@ Fixpoint closedn k (t : term) : bool :=
   | tProj p c => closedn k c
   | tFix mfix idx =>
     let k' := List.length mfix + k in
-    List.forallb (test_def (closedn k')) mfix
+    List.forallb (test_def (closedn k) (closedn k')) mfix
   | tCoFix mfix idx =>
     let k' := List.length mfix + k in
-    List.forallb (test_def (closedn k')) mfix
+    List.forallb (test_def (closedn k) (closedn k')) mfix
   | x => true
   end.
 
@@ -97,10 +104,13 @@ Notation closed t := (closedn 0 t).
 
 Create HintDb terms.
 
+Ltac arith_congr := repeat (try lia; progress f_equal).
+
 Ltac easy0 :=
   let rec use_hyp H :=
    (match type of H with
     | _ /\ _ => exact H || destruct_hyp H
+    | _ * _ => exact H || destruct_hyp H
     | _ => try (solve [ inversion H ])
     end)
   with do_intro := (let H := fresh in
@@ -110,32 +120,35 @@ Ltac easy0 :=
   let rec use_hyps :=
    (match goal with
     | H:_ /\ _ |- _ => exact H || (destruct_hyp H; use_hyps)
+    | H:_ * _ |- _ => exact H || (destruct_hyp H; use_hyps)
     | H:_ |- _ => solve [ inversion H ]
     | _ => idtac
     end)
   in
-  let do_atom := (solve [ trivial with eq_true | reflexivity | symmetry; trivial | contradiction ]) in
-  let rec do_ccl := (try do_atom; repeat (do_intro; try do_atom); (solve [ split; do_ccl ])) in
+  let do_atom := (solve [ trivial with eq_true | reflexivity | symmetry; trivial | contradiction | congruence]) in
+  let rec do_ccl := (try do_atom; repeat (do_intro; try do_atom); try arith_congr; (solve [ split; do_ccl ])) in
   (solve [ do_atom | use_hyps; do_ccl ]) || fail "Cannot solve this goal".
-Require Import Omega.
-Hint Extern 100 => omega : terms.
 
-Ltac easy ::= easy0 || solve [eauto 7 with core arith terms].
 
-Notation lift_rec n c k := (lift n k c) (only parsing).
+Hint Extern 10 (_ < _)%nat => lia : terms.
+Hint Extern 10 (_ <= _)%nat => lia : terms.
+Hint Extern 10 (@eq nat _ _) => lia : terms.
+
+Ltac easy ::= easy0 || solve [intuition eauto 3 with core terms].
+
 Notation subst_rec N M k := (subst N k M) (only parsing).
 
 Require Import PeanoNat.
 Import Nat.
 
 Lemma lift_rel_ge :
-  forall k n p, p <= n -> lift_rec k (tRel n) p = tRel (k + n).
+  forall k n p, p <= n -> lift k p (tRel n) = tRel (k + n).
 Proof.
   intros; simpl in |- *.
   now elim (leb_spec p n).
 Qed.
 
-Lemma lift_rel_lt : forall k n p, p > n -> lift_rec k (tRel n) p = tRel n.
+Lemma lift_rel_lt : forall k n p, p > n -> lift k p (tRel n) = tRel n.
 Proof.
   intros; simpl in |- *.
   now elim (leb_spec p n).
@@ -146,113 +159,155 @@ Proof.
   intros; simpl. now destruct leb.
 Qed.
 
-Lemma subst_rel_lt : forall u n k, k > n -> subst_rec u (tRel n) k = tRel n.
+Lemma subst_rel_lt : forall u n k, k > n -> subst u k (tRel n) = tRel n.
 Proof.
   simpl in |- *; intros.
-  elim (compare_spec k n); intro Hcomp; easy.
+  elim (leb_spec k n); intro Hcomp; easy.
 Qed.
 
 Lemma subst_rel_gt :
-  forall u n k, n > k -> subst_rec u (tRel n) k = tRel (pred n).
+  forall u n k, n >= k + length u -> subst u k (tRel n) = tRel (n - length u).
 Proof.
   simpl in |- *; intros.
-  now elim (compare_spec k n). 
+  elim (leb_spec k n). intros. destruct nth_error eqn:Heq.
+  assert (n - k < length u) by (apply nth_error_Some; congruence). lia. reflexivity.
+  lia.
 Qed.
 
-Lemma subst_rel_eq : forall u n, subst_rec u (tRel n) n = lift0 n u.
+Lemma subst_rel_eq :
+  forall (u : list term) n i t p,
+    List.nth_error u i = Some t -> p = n + i ->
+    subst u n (tRel p) = lift0 n t.
 Proof.
-  intros; simpl in |- *.
-  now elim (compare_spec n n).
+  intros; simpl in |- *. subst p.
+  elim (leb_spec n (n + i)). intros. assert (n + i - n = i) by lia. rewrite H1, H.
+  reflexivity. intros. lia.
 Qed.
 
-Lemma lift_rec0 : forall M k, lift_rec 0 M k = M.
+Hint Extern 0 (_ = _) => progress f_equal : all.
+Hint Unfold on_snd snd : all.
+
+Lemma on_snd_eq_id_spec {A B} (f : B -> B) (x : A * B) :
+  f (snd x) = snd x <->
+  on_snd f x = x.
+Proof.
+  destruct x; simpl; unfold on_snd; simpl. split; congruence.
+Qed.
+Hint Resolve -> on_snd_eq_id_spec : all.
+
+Lemma map_def_eq_spec {A B : Set} (f f' g g' : A -> B) (x : def A) :
+  f (dtype x) = g (dtype x) ->
+  f' (dbody x) = g' (dbody x) ->
+  map_def f f' x = map_def g g' x.
+Proof.
+  intros. unfold map_def; f_equal; auto.
+Qed.
+Hint Resolve map_def_eq_spec : all.
+
+Lemma map_def_id_spec {A : Set} (f f' : A -> A) (x : def A) :
+  f (dtype x) = (dtype x) ->
+  f' (dbody x) = (dbody x) ->
+  map_def f f' x = x.
+Proof.
+  intros. rewrite (map_def_eq_spec _ _ id id); auto. destruct x; auto.
+Qed.
+Hint Resolve map_def_id_spec : all.
+
+Hint Extern 10 (_ < _)%nat => lia : all.
+Hint Extern 10 (_ <= _)%nat => lia : all.
+Hint Extern 10 (@eq nat _ _) => lia : all.
+
+Ltac change_Sk :=
+  repeat match goal with
+    |- context [S (?x + ?y)] => progress change (S (x + y)) with (S x + y)
+  end.
+
+Ltac all_simpl :=
+  progress (unfold compose; simpl).
+
+Hint Extern 10 => all_simpl : all.
+
+Ltac solve_all :=
+  unfold tCaseBrsProp, tFixProp in *;
+  repeat toAll; try All_map; try close_Forall;
+  change_Sk; auto with all;
+  intuition eauto 4 with all.
+
+Ltac nth_leb_simpl :=
+  match goal with
+    |- context [leb ?k ?n] => elim (leb_spec_Set k n); try lia; intros; simpl
+  | |- context [nth_error ?l ?n] => elim (nth_error_spec l n); rewrite -> ?app_length, ?map_length;
+                                    try lia; intros; simpl
+  | H : context[nth_error (?l ++ ?l') ?n] |- _ =>
+    (rewrite -> (AstUtils.nth_error_app_ge l l' n) in H by lia) ||
+    (rewrite -> (AstUtils.nth_error_app_lt l l' n) in H by lia)
+  | H : nth_error ?l ?n = Some _, H' : nth_error ?l ?n' = Some _ |- _ =>
+    replace n' with n in H' by lia; rewrite -> H in H'; injection H'; intros; subst
+  | _ => lia || congruence || solve [repeat (f_equal; try lia)]
+  end.
+
+Lemma lift0_id : forall M k, lift 0 k M = M.
 Proof.
   intros M.
   elim M using term_forall_list_ind; simpl in |- *; intros; try easy ;
-    try (try rewrite H; try rewrite H0 ; try rewrite H1 ; easy).
+    try (try rewrite H; try rewrite H0 ; try rewrite H1 ; easy);
+    try (f_equal; auto; solve_all).
 
   - now elim (leb k n).
-  - f_equal. rewrite <- map_id. now eapply (forall_map_spec H).
-  - f_equal. auto. rewrite <- map_id. now eapply (forall_map_spec H0).
-  - f_equal; auto. rewrite <- map_id. eapply (forall_map_spec H1).
-    intros. destruct x; unfold on_snd. simpl. rewrite H2. reflexivity.
-
-  - f_equal. transitivity (map (map_def id) m). eapply (tfix_map_spec H); auto.
-    rewrite <- map_id. f_equal. extensionality x. destruct x; reflexivity.
-  - f_equal. transitivity (map (map_def id) m). eapply (tfix_map_spec H); auto.
-    rewrite <- map_id. f_equal. extensionality x. destruct x; reflexivity.
 Qed.
 
 Lemma lift0_p : forall M, lift0 0 M = M.
   intros; unfold lift in |- *.
-  apply lift_rec0; easy.
+  apply lift0_id; easy.
 Qed.
 
+Hint Extern 10 => progress unfold compose : all.
 
-Lemma simpl_lift_rec :
+Hint Extern 10 => apply_spec : all.
+
+Hint Resolve -> on_snd_eq_spec : all.
+
+Lemma simpl_lift :
   forall M n k p i,
     i <= k + n ->
-    k <= i -> lift_rec p (lift_rec n M k) i = lift_rec (p + n) M k.
+    k <= i -> lift p i (lift n k M) = lift (p + n) k M.
 Proof.
   intros M.
   elim M using term_forall_list_ind;
-    intros; simpl; try easy;
-      rewrite ?map_map_compose, ?compose_on_snd, ?compose_map_def;
-      try (rewrite H, ?H0, ?H1; auto); try (f_equal; apply_spec);
-        try rewrite ?map_length; try easy.
+    intros; simpl;
+      rewrite -> ?map_map_compose, ?compose_on_snd, ?compose_map_def, ?map_length;
+      try (rewrite -> H, ?H0, ?H1; auto); try (f_equal; auto; solve_all).
 
   - elim (leb_spec k n); intros.
     now rewrite lift_rel_ge.
     now rewrite lift_rel_lt.
 Qed.
 
-Lemma simpl_lift : forall M n, lift0 (S n) M = lift0 1 (lift0 n M).
-  now intros; rewrite simpl_lift_rec.
-Qed.
-
-Lemma permute_lift_rec :
-  forall M n k p i,
-    i <= k ->
-    lift_rec p (lift_rec n M k) i = lift_rec n (lift_rec p M i) (p + k).
-Proof.
-  intros M.
-  elim M using term_forall_list_ind;
-    intros; simpl; try easy;
-      rewrite ?map_map_compose, ?compose_on_snd, ?compose_map_def;
-      try solve [f_equal; easy];
-      try (f_equal; try easy; apply_spec);
-      unfold compose; intros;
-        try rewrite ?map_length; try easy ;
-        try (rewrite H, H0; f_equal; try easy; now f_equal);
-        try (rewrite H, H0, H1; f_equal; try easy; now f_equal);
-        try (rewrite H1; now f_equal).
-  
-  - elim (leb_spec k n); intros;
-    elim (leb_spec i n); intros; try easy.
-    + rewrite 2!lift_rel_ge; try easy.
-    + rewrite lift_rel_ge, lift_rel_lt; try easy.
-    + rewrite 2!lift_rel_lt; try easy.
+Lemma simpl_lift0 : forall M n, lift0 (S n) M = lift0 1 (lift0 n M).
+  now intros; rewrite simpl_lift.
 Qed.
 
 Lemma permute_lift :
-  forall M k, lift0 1 (lift_rec 1 M k) = lift_rec 1 (lift0 1 M) (S k).
+  forall M n k p i,
+    i <= k ->
+    lift p i (lift n k M) = lift n (k + p) (lift p i M).
+Proof.
+  intros M.
+  elim M using term_forall_list_ind;
+    intros; simpl;
+      rewrite -> ?map_map_compose, ?compose_on_snd, ?compose_map_def, ?map_length, ?Nat.add_assoc;
+      try solve [f_equal; auto; solve_all]; repeat nth_leb_simpl.
+Qed.
+
+Lemma permute_lift0 :
+  forall M k, lift0 1 (lift 1 k M) = lift 1 (S k) (lift0 1 M).
   intros.
-  change (lift_rec 1 (lift_rec 1 M k) 0 = lift_rec 1 (lift_rec 1 M 0) (1 + k))
+  change (lift 1 0 (lift 1 k M) = lift 1 (1 + k) (lift 1 0 M))
     in |- *.
-  apply permute_lift_rec; easy.
+  rewrite permute_lift; easy.
 Qed.
 
-Lemma Forall_map {A B} (P : B -> Prop) (f : A -> B) l : Forall (Program.Basics.compose P f) l -> Forall P (map f l).
-Proof.
-  induction 1; constructor; auto.
-Qed.
-
-Lemma Forall_impl {A} (P Q : A -> Prop) : forall l, Forall P l -> (forall x, P x -> Q x) -> Forall Q l.
-Proof.
-  induction 1; constructor; auto.
-Qed.
-
-Lemma lift_rec_isApp n k t : ~ isApp t = true -> ~ isApp (lift n k t) = true.
+Lemma lift_isApp n k t : ~ isApp t = true -> ~ isApp (lift n k t) = true.
 Proof.
   induction t; auto.
   intros.
@@ -266,161 +321,89 @@ Proof.
   contradiction.
 Qed.
 
-Lemma lift_rec_wf n k t : wf t -> wf (lift_rec n t k).
-Proof.
-  intros wft; revert t wft k.
-  apply (term_wf_forall_list_ind (fun t => forall k, wf (lift n k t))) ; simpl; intros; try constructor; auto.
-  destruct leb; constructor.
-  apply Forall_map.
-  induction H; constructor; auto.
-  now apply lift_rec_isApp.
-  now apply map_non_nil.
-  apply Forall_map. eapply Forall_impl. apply H2. auto.
-  apply Forall_map. eapply Forall_impl. apply H1.
-  intros [n' t]. simpl. repeat red; simpl; auto.
-  apply Forall_map. eapply Forall_impl. apply H.
-  simpl. intros. red; intuition (simpl; auto).
-  apply Forall_map. eapply Forall_impl. apply H.
-  simpl. intros. red; intuition (simpl; auto).
-Qed.
+Lemma isLambda_lift n k (bod : term) :
+  isLambda bod = true -> isLambda (lift n k bod) = true.
+Proof. destruct bod; simpl; try congruence. Qed.
 
-Lemma mkApps_tApp t l :
-  ~ isApp t = true -> l <> nil -> mkApps t l = tApp t l.
-Proof.
-  intros.
-  destruct l. simpl. contradiction.
-  destruct t; simpl; try reflexivity.
-  simpl in H. contradiction.
-Qed.
+Hint Resolve lift_isApp map_non_nil isLambda_lift : all.
 
 Hint Unfold compose.
 Hint Transparent compose.
 
 Lemma simpl_subst_rec :
-  forall M (H : wf M) N n p k,
+  forall M N n p k,
     p <= n + k ->
-    k <= p -> subst_rec N (lift_rec (S n) M k) p = lift_rec n M k.
+    k <= p -> subst N p (lift (List.length N + n) k M) = lift n k M.
 Proof.
-  intros M wfM. induction wfM using term_wf_forall_list_ind;
-    intros; simpl; try easy;
-      rewrite ?map_map_compose, ?compose_on_snd, ?compose_map_def;
-      try solve [f_equal; easy];
-      try (f_equal; try easy; apply_spec); intros;
-        try rewrite ?map_length; try easy ||
-      (try rewrite H, H0; f_equal; try easy; now f_equal).
-  
-  - elim (leb_spec k n); intros; try easy.
-    + rewrite subst_rel_gt; try easy.
-    + rewrite subst_rel_lt; try easy.
-
-  - rewrite IHwfM; auto.
-    apply (lift_rec_isApp n k) in H.
-    rewrite mkApps_tApp; auto using map_non_nil.
-    f_equal. eapply forall_map_spec. apply H1; simpl; auto.
-    simpl; intros. typeclasses eauto with core.
+  intros M. induction M using term_forall_list_ind;
+    intros; simpl;
+      rewrite -> ?map_map_compose, ?compose_on_snd, ?compose_map_def, ?map_length;
+      try solve [f_equal; auto; solve_all]; repeat nth_leb_simpl.
 Qed.
 
 Lemma simpl_subst :
-  forall N M (H : wf M) n p, p <= n -> subst_rec N (lift0 (S n) M) p = lift0 n M.
-  intros; now apply simpl_subst_rec.
-Qed.
-
-Lemma mkApps_tRel n a l : mkApps (tRel n) (a :: l) = tApp (tRel n) (a :: l).
-Proof.
-  simpl. reflexivity.
-Qed.
+  forall N M n p, p <= n -> subst N p (lift0 (length N + n) M) = lift0 n M.
+Proof. intros. rewrite simpl_subst_rec; auto. now rewrite Nat.add_0_r. lia. Qed.
 
 Lemma lift_mkApps n k t l : lift n k (mkApps t l) = mkApps (lift n k t) (map (lift n k) l).
 Proof.
-  revert n k t; induction l; intros n k t; destruct t; try reflexivity.
-  rewrite lift_rel_alt. rewrite !mkApps_tRel.
-  simpl lift.
-  simpl map. rewrite !mkApps_tRel.
-  f_equal. destruct leb; auto.
-
-  simpl. f_equal.
-  now rewrite map_app.
+  revert n k t; induction l; intros n k t. auto.
+  simpl. rewrite (IHl n k (tApp t a)). reflexivity.
 Qed.
 
 Lemma commut_lift_subst_rec :
   forall M N n p k,
     k <= p ->
-    lift_rec n (subst_rec N M p) k = subst_rec N (lift_rec n M k) (n + p).
+    lift n k (subst N p M) = subst N (p + n) (lift n k M).
 Proof.
   intros M.
   elim M using term_forall_list_ind;
     intros; simpl; try easy;
-      rewrite ?map_map_compose, ?compose_on_snd, ?compose_map_def;
-      try solve [f_equal; easy];
-      try (f_equal; try easy; apply_spec);
-      unfold compose; intros;
-        try rewrite ?map_length; try easy ;
-        try (rewrite H, H0; f_equal; try easy; now f_equal);
-        try (rewrite H, H0, H1; f_equal; try easy; now f_equal);
-        try (rewrite H1; now f_equal).
-  
-  - elim (compare_spec p n); elim (leb_spec k n); intros; subst; try easy.
-    + rewrite subst_rel_eq; try easy.
-      now rewrite simpl_lift_rec.
-    + rewrite subst_rel_gt; try easy.
-      now rewrite lift_rel_ge.
-    + rewrite lift_rel_ge; try easy.
-      now rewrite subst_rel_lt.
-    + rewrite lift_rel_lt; try easy.
-      now rewrite subst_rel_lt.
+      rewrite -> ?map_map_compose, ?compose_on_snd, ?compose_map_def, ?map_length, ?Nat.add_assoc;
+      try solve [f_equal; auto; solve_all].
 
-  - rewrite lift_mkApps. f_equal. auto.
-    rewrite map_map_compose. apply_spec. intros.
-    now apply H2.
+  - repeat nth_leb_simpl.
+    rewrite -> simpl_lift by easy. f_equal; lia.
 Qed.
 
 Lemma commut_lift_subst :
-  forall M N k, subst_rec N (lift0 1 M) (S k) = lift0 1 (subst_rec N M k).
+  forall M N k, subst N (S k) (lift0 1 M) = lift0 1 (subst N k M).
   now intros; rewrite commut_lift_subst_rec.
 Qed.
 
 Lemma distr_lift_subst_rec :
   forall M N n p k,
-    lift_rec n (subst_rec N M p) (p + k) =
-    subst_rec (lift_rec n N k) (lift_rec n M (S (p + k))) p.
+    lift n (p + k) (subst N p M) =
+    subst (List.map (lift n k) N) p (lift n (p + length N + k) M).
 Proof.
   intros M.
   elim M using term_forall_list_ind;
     intros; match goal with
               |- context [tRel _] => idtac
-            | |- _ => simpl
+            | |- _ => cbn -[plus]
             end; try easy;
-      rewrite ?map_map_compose, ?compose_on_snd, ?compose_map_def;
-      try solve [f_equal; easy];
-      try (f_equal; try easy; apply_spec);
-      unfold compose; intros;
-        try rewrite ?map_length; try easy ;
-        try (erewrite H, <- H0; f_equal; try easy; now f_equal);
-        try (erewrite H, <- H0, <- H1; f_equal; try easy; now f_equal);
-        try (erewrite H1; now f_equal).
-  
-  - unfold subst at 1. unfold lift at 4.
-    elim (compare_spec p n); intros; try easy;
-    elim (leb_spec (S (p + k)) n); intros; subst; try easy.
-    
-    + rewrite subst_rel_eq. now rewrite <- permute_lift_rec. 
-    + rewrite lift_rel_ge; try easy.
-      now rewrite subst_rel_gt.
-    + rewrite lift_rel_lt; try easy.
-      now rewrite subst_rel_gt.
-    + rewrite lift_rel_lt; try easy.
-      now rewrite subst_rel_lt.
+      rewrite -> ?map_map_compose, ?compose_on_snd, ?compose_map_def, ?map_length, ?Nat.add_assoc;
+      try solve [f_equal; auto; solve_all].
 
-  - rewrite lift_mkApps. f_equal; auto.
-    rewrite map_map_compose; apply_spec; simpl.
-    intros. apply H1.
-  - rewrite add_assoc, H0. f_equal. now f_equal.
-  - rewrite add_assoc, H0. f_equal. now f_equal.
+  - unfold subst at 1. unfold lift at 4.
+    repeat nth_leb_simpl.
+    rewrite nth_error_map in e0. rewrite e in e0.
+    revert e0. intros [= <-].
+    now rewrite (permute_lift x n0 k p 0).
 Qed.
 
 Lemma distr_lift_subst :
   forall M N n k,
-    lift_rec n (subst0 N M) k = subst0 (lift_rec n N k) (lift_rec n M (S k)).
+    lift n k (subst0 N M) = subst0 (map (lift n k) N) (lift n (length N + k) M).
+Proof.
+  intros. pattern k at 1 3 in |- *.
+  replace k with (0 + k); try easy.
+  apply distr_lift_subst_rec.
+Qed.
+
+Lemma distr_lift_subst10 :
+  forall M N n k,
+    lift n k (subst10 N M) = subst10 (lift n k N) (lift n (S k) M).
 Proof.
   intros; unfold subst in |- *.
   pattern k at 1 3 in |- *.
@@ -428,23 +411,23 @@ Proof.
   apply distr_lift_subst_rec.
 Qed.
 
-Lemma mkApp_nested f l l' : mkApps (mkApps f l) l' = mkApps f (l ++ l').
+Lemma subst_mkApps u k t l :
+  subst u k (mkApps t l) = mkApps (subst u k t) (map (subst u k) l).
 Proof.
-  induction l; destruct f; destruct l'; simpl; rewrite ?app_nil_r; auto.
-  f_equal. now rewrite <- app_assoc.
+  revert u k t; induction l; intros u k t; auto.
+  intros. simpl mkApps at 1. simpl subst at 1 2.
+  now rewrite IHl.
 Qed.
 
-Lemma subst_mkApps u k t l : subst u k (mkApps t l) = mkApps (subst u k t) (map (subst u k) l).
+Lemma subst1_mkApps u k t l : subst1 u k (mkApps t l) = mkApps (subst1 u k t) (map (subst1 u k) l).
 Proof.
-  revert u k t; induction l; intros u k t; destruct t; try reflexivity.
-  intros. simpl mkApps at 1. simpl subst at 2. simpl subst at 1.
-  rewrite map_app. now rewrite mkApp_nested.
+  apply subst_mkApps.
 Qed.
 
 Lemma distr_subst_rec :
-  forall M N (P : term) (wfP : wf P) n p,
-    subst_rec P (subst_rec N M p) (p + n) =
-    subst_rec (subst_rec P N n) (subst_rec P M (S (p + n))) p.
+  forall M N (P : list term) n p,
+    subst P (p + n) (subst N p M) =
+    subst (map (subst P n) N) p (subst P (p + length N + n) M).
 Proof.
   intros M.
   elim M using term_forall_list_ind;
@@ -452,73 +435,122 @@ Proof.
               |- context [tRel _] => idtac
             | |- _ => simpl
             end; try easy;
-      rewrite ?map_map_compose, ?compose_on_snd, ?compose_map_def;
-      try solve [f_equal; easy];
-      try (f_equal; try easy; apply_spec);
-      unfold compose; intros;
-        try rewrite ?map_length; try easy ;
-        try (erewrite H, <- H0; f_equal; try easy; now f_equal);
-        try (erewrite H, <- H0, <- H1; f_equal; try easy; now f_equal);
-        try (erewrite H1; now f_equal).
-  
-  - unfold subst at 2. 
-    elim (compare_spec p n); intros; try easy.
-    
-    + subst. rewrite subst_rel_lt; try easy.
-      rewrite subst_rel_eq; try easy.
-      now rewrite <- commut_lift_subst_rec.
-    + unfold subst at 4.
-      elim (compare_spec (S (p + n0)) n); intros; subst; try easy.
-      ++ rewrite subst_rel_eq.
-         now rewrite simpl_subst_rec.
-      ++ rewrite !subst_rel_gt; try easy.
-      ++ rewrite subst_rel_lt; try easy.
-         now rewrite subst_rel_gt.
-    + rewrite !subst_rel_lt; try easy.
+      rewrite -> ?map_map_compose, ?compose_on_snd, ?compose_map_def, ?map_length, ?Nat.add_assoc;
+      try solve [f_equal; auto; solve_all].
 
-  - rewrite !subst_mkApps. rewrite H; auto. f_equal.
-    rewrite !map_map_compose. apply_spec. intros.
-    unfold compose. auto.
-  - rewrite add_assoc, H0; auto. f_equal. now f_equal.
-  - rewrite add_assoc, H0; auto. f_equal. now f_equal.
+  - unfold subst at 2.
+    repeat nth_leb_simpl.
+    erewrite <- simpl_subst. f_equal. rewrite map_length. arith_congr. lia.
+    rewrite nth_error_map in e0. rewrite e in e0.
+    simpl in e0. injection e0 as <-.
+    rewrite commut_lift_subst_rec. arith_congr. lia.
 Qed.
 
 Lemma distr_subst :
-  forall (P : term) (wfP : wf P) N M k,
-    subst_rec P (subst0 N M) k = subst0 (subst_rec P N k) (subst_rec P M (S k)).
+  forall P N M k,
+    subst P k (subst0 N M) = subst0 (map (subst P k) N) (subst P (length N + k) M).
 Proof.
-  intros; unfold subst in |- *.
+  intros.
   pattern k at 1 3 in |- *.
-  change k with (0 + k).
-  now apply distr_subst_rec.
+  change k with (0 + k). hnf.
+  apply distr_subst_rec.
 Qed.
 
-
-Lemma lift_closed n k t : closedn k t = true -> lift n k t = t.
+Lemma lift_closed n k t : closedn k t -> lift n k t = t.
 Proof.
   revert k.
   elim t using term_forall_list_ind; intros; try easy;
-    rewrite ?map_map_compose, ?compose_on_snd, ?compose_map_def;
-    try (f_equal; apply_spec);  simpl closed in *;
-    try rewrite ?map_length; try easy.
+    rewrite -> ?map_map_compose, ?compose_on_snd, ?compose_map_def, ?map_length;
+    unfold test_def in *;
+    simpl closed in *; try solve [simpl lift; simpl closed; f_equal; auto; toProp; solve_all]; try easy.
   - rewrite lift_rel_lt; auto.
     revert H. elim (Nat.ltb_spec n0 k); intros; try easy.
-  - simpl lift; f_equal.
-    rewrite <- map_id. 
-    apply_spec; eauto.
-  - simpl lift. rewrite andb_true_iff in H1. f_equal; intuition eauto.
-  - simpl lift; rewrite andb_true_iff in H1. f_equal; intuition eauto.
-  - simpl lift. rewrite !andb_true_iff in H2. f_equal; intuition eauto.
-  - simpl lift. rewrite !andb_true_iff in H1. f_equal; intuition eauto.
-    rewrite <- map_id; apply_spec; eauto.
-  - simpl lift. rewrite !andb_true_iff in H2. f_equal; intuition eauto.
-    transitivity (map (on_snd id) l). apply_spec; eauto.
-    rewrite <- map_id. f_equal. unfold on_snd. extensionality p. now destruct p.
-  - simpl lift. f_equal; eauto.
-  - simpl lift. f_equal.
-    transitivity (map (map_def id) m). apply_spec; eauto.
-    now autorewrite with core.
-  - simpl lift. f_equal.
-    transitivity (map (map_def id) m). apply_spec; eauto.
-    now autorewrite with core.
+  - simpl lift. f_equal. solve_all. unfold test_def in b. toProp. solve_all.
+  - simpl lift. f_equal. solve_all. unfold test_def in b. toProp. solve_all.
+Qed.
+
+Lemma closed_upwards {k t} k' : closedn k t -> k' >= k -> closedn k' t.
+Proof.
+  revert k k'.
+  elim t using term_forall_list_ind; intros; try lia;
+    rewrite -> ?map_map_compose, ?compose_on_snd, ?compose_map_def, ?map_length;
+    simpl closed in *; unfold test_snd, test_def in *;
+      try solve [(try f_equal; simpl; repeat (toProp; solve_all); eauto)].
+
+  - elim (ltb_spec n k'); auto. intros.
+    apply ltb_lt in H. lia.
+Qed.
+
+Lemma subst_empty k a : subst [] k a = a.
+Proof.
+  induction a in k |- * using term_forall_list_ind; simpl; try congruence;
+    try solve [f_equal; eauto; solve_all].
+
+  - elim (Nat.compare_spec k n); destruct (Nat.leb_spec k n); intros; try easy.
+    subst. rewrite Nat.sub_diag. simpl. rewrite Nat.sub_0_r. reflexivity.
+    assert (n - k > 0) by lia.
+    assert (exists n', n - k = S n'). exists (pred (n - k)). lia.
+    destruct H2. rewrite H2. simpl. now rewrite Nat.sub_0_r.
+Qed.
+
+(* Lemma lift_to_extended_list_k Γ k : forall k', *)
+(*  to_extended_list_k Γ (k' + k) = map (lift0 k') (to_extended_list_k Γ k). *)
+(* Proof. *)
+(*   unfold to_extended_list_k. *)
+(*   intros k'. rewrite !reln_alt_eq, !app_nil_r. *)
+(*   induction Γ in k, k' |- *; simpl; auto. *)
+(*   destruct a as [na [body|] ty]. *)
+(*   now rewrite <- Nat.add_assoc, (IHΓ (k + 1) k'). *)
+(*   simpl. now rewrite <- Nat.add_assoc, (IHΓ (k + 1) k'), map_app. *)
+(* Qed. *)
+
+Lemma simpl_subst_k (N : list term) (M : term) :
+  forall k p, p = #|N| -> subst N k (lift p k M) = M.
+Proof.
+  intros. subst p. rewrite <- (Nat.add_0_r #|N|).
+  rewrite -> simpl_subst_rec, lift0_id; auto.
+Qed.
+
+Lemma subst_app_decomp l l' k t :
+  subst (l ++ l') k t = subst l' k (subst (List.map (lift0 (length l')) l) k t).
+Proof.
+  induction t in k |- * using term_forall_list_ind; simpl; auto;
+    rewrite ?subst_mkApps; try change_Sk;
+    try (f_equal; rewrite -> ?map_map_compose, ?compose_on_snd, ?compose_map_def, ?map_length;
+         eauto; solve_all).
+
+  - repeat nth_leb_simpl.
+    rewrite nth_error_map in e0. rewrite e in e0.
+    injection e0; intros <-.
+    rewrite -> permute_lift by auto.
+    rewrite <- (Nat.add_0_r #|l'|).
+    rewrite -> simpl_subst_rec, lift0_id; auto with wf; try lia.
+Qed.
+
+Lemma subst_app_simpl l l' k t :
+  subst (l ++ l') k t = subst l k (subst l' (k + length l) t).
+Proof.
+  induction t in k |- * using term_forall_list_ind; simpl; eauto;
+    rewrite ?subst_mkApps; try change_Sk;
+    try (f_equal; rewrite -> ?map_map_compose, ?compose_on_snd, ?compose_map_def, ?map_length, ?Nat.add_assoc;
+         eauto; solve_all; eauto).
+
+  - repeat nth_leb_simpl.
+    rewrite -> Nat.add_comm, simpl_subst; eauto.
+Qed.
+
+Lemma isLambda_subst (s : list term) k (bod : term) :
+  isLambda bod = true -> isLambda (subst s k bod) = true.
+Proof.
+  intros. destruct bod; try discriminate. reflexivity.
+Qed.
+
+Lemma map_vass_map_def g l n k :
+  (mapi (fun i (d : def term) => vass (dname d) (lift0 i (dtype d)))
+        (map (map_def (lift n k) g) l)) =
+  (mapi (fun i d => map_decl (lift n (i + k)) d) (mapi (fun i (d : def term) => vass (dname d) (lift0 i (dtype d))) l)).
+Proof.
+  rewrite mapi_mapi, mapi_map. apply mapi_ext.
+  intros. unfold map_decl, vass; simpl; f_equal.
+  rewrite permute_lift. f_equal; lia. lia.
 Qed.
