extraction/theories/Typing.v
@@ -1,8 +1,8 @@
 (* Distributed under the terms of the MIT license.   *)
 
 From Coq Require Import Bool String List Program BinPos Compare_dec Omega.
-Require Import Template.config Template.utils Template.kernel.univ.
-From TemplateExtraction Require Import Ast Induction LiftSubst UnivSubst.
+From Template Require Import config utils kernel.univ AstUtils.
+From TemplateExtraction Require Import Ast AstUtils Induction LiftSubst UnivSubst.
 Require Import String.
 Local Open Scope string_scope.
 Set Asymmetric Patterns.
@@ -15,7 +15,6 @@ Set Asymmetric Patterns.
   Inductive relations for reduction, conversion and typing of CIC terms.
 
  *)
-
 (** ** Environment lookup *)
 
 Definition global_decl_ident d :=
@@ -23,32 +22,6 @@ Definition global_decl_ident d :=
   | ConstantDecl id _ => id
   | InductiveDecl id _ => id
   end.
-
-Definition is_constant_decl d :=
-  match d with
-  | InductiveDecl _ _ => false
-  | _ => true
-  end.
-
-Definition is_minductive_decl d :=
-  match d with
-  | InductiveDecl _ _ => true
-  | _ => false
-  end.
-
-Definition is_inductive_decl_for i d :=
-  match d with
-  | InductiveDecl _ cb => i < List.length cb.(ind_bodies)
-  | _ => False
-  end.
-
-Definition ident_eq (x y : ident) :=
-  if string_dec x y then true else false.
-
-Lemma ident_eq_spec x y : reflect (x = y) (ident_eq x y).
-Proof.
-  unfold ident_eq. destruct string_dec; constructor; auto.
-Qed.
 
 Fixpoint lookup_env (Σ : global_declarations) (id : ident) : option global_decl :=
   match Σ with
@@ -64,43 +37,19 @@ Definition declared_constant (Σ : global_declarations) (id : ident) decl : Prop
 Definition declared_minductive Σ mind decl :=
   lookup_env Σ mind = Some (InductiveDecl mind decl).
 
-Definition declared_inductive Σ ind univs decl :=
-  exists decl', declared_minductive Σ (inductive_mind ind) decl' /\
-                univs = decl'.(ind_universes) /\
-                List.nth_error decl'.(ind_bodies) (inductive_ind ind) = Some decl.
+Definition declared_inductive Σ mdecl ind decl :=
+  declared_minductive Σ (inductive_mind ind) mdecl /\
+  List.nth_error mdecl.(ind_bodies) (inductive_ind ind) = Some decl.
 
-Definition declared_constructor Σ cstr univs decl : Prop :=
-  let '(ind, k) := cstr in
-  exists decl', declared_inductive Σ ind univs decl' /\
-                List.nth_error decl'.(ind_ctors) k = Some decl.
+Definition declared_constructor Σ mdecl idecl cstr cdecl : Prop :=
+  declared_inductive Σ mdecl (fst cstr) idecl /\
+  List.nth_error idecl.(ind_ctors) (snd cstr) = Some cdecl.
 
-Definition declared_projection Σ (proj : projection) decl : Prop :=
-  let '(ind, ppars, arg) := proj in
-  exists univs decl', declared_inductive Σ ind univs decl' /\
-                List.nth_error decl'.(ind_projs) arg = Some decl.
+Definition declared_projection Σ mdecl idecl (proj : projection) pdecl : Prop :=
+  declared_inductive Σ mdecl (fst (fst proj)) idecl /\
+  List.nth_error idecl.(ind_projs) (snd proj) = Some pdecl.
 
-Program
-Definition type_of_constant_decl (d : global_decl | is_constant_decl d = true) : term :=
-  match d with
-  | InductiveDecl _ _ => !
-  | ConstantDecl _ decl => decl.(cst_type)
-  end.
-
-Program
-Definition body_of_constant_decl (d : global_decl | is_constant_decl d = true) : option term :=
-  match d with
-  | InductiveDecl _ _ => !
-  | ConstantDecl _ decl => decl.(cst_body)
-  end.
-
-Program
-Definition types_of_minductive_decl (d : global_decl | is_minductive_decl d = true) :
-  list one_inductive_body :=
-  match d with
-  | InductiveDecl _ tys => tys.(ind_bodies)
-  | ConstantDecl _ _ => !
-  end.
-
+(** Inductive substitution, to produce a constructors' type *)
 Definition inds ind u (l : list one_inductive_body) :=
   let fix aux n :=
       match n with
@@ -109,23 +58,11 @@ Definition inds ind u (l : list one_inductive_body) :=
       end
   in aux (List.length l).
 
-Program
-Definition type_of_constructor (Σ : global_declarations) (c : inductive * nat) (univs : universe_context) (u : list Level.t) (decl : ident * term * nat)
-           (H : declared_constructor Σ c univs decl) :=
-  let mind := inductive_mind (fst c) in
-  let '(id, trm, args) := decl in
-  match lookup_env Σ mind with
-  | Some (InductiveDecl _ decl') =>
-    substl (inds mind u decl'.(ind_bodies)) (subst_instance_constr u trm)
-  | _ => !
-  end.
+Lemma inds_length ind u l : #|inds ind u l| = #|l|.
+Proof.
+  unfold inds. induction l; simpl; congruence.
+Qed.
 
-Next Obligation.
-  destruct H as [decl [H H']].
-  destruct H as [decl' [H'' H''']].
-  eapply H0.
-  simpl. rewrite H''. reflexivity.
-Defined.
 
 (** ** Reduction *)
 
@@ -141,24 +78,54 @@ Definition fix_subst (l : mfixpoint term) :=
 
 Definition unfold_fix (mfix : mfixpoint term) (idx : nat) :=
   match List.nth_error mfix idx with
-  | Some d => Some (d.(rarg), substl (fix_subst mfix) d.(dbody))
+  | Some d => Some (d.(rarg), subst0 (fix_subst mfix) d.(dbody))
+  | None => None
+  end.
+
+Definition cofix_subst (l : mfixpoint term) :=
+  let fix aux n :=
+      match n with
+      | 0 => []
+      | S n => tCoFix l n :: aux n
+      end
+  in aux (List.length l).
+
+Definition unfold_cofix (mfix : mfixpoint term) (idx : nat) :=
+  match List.nth_error mfix idx with
+  | Some d => Some (d.(rarg), subst0 (cofix_subst mfix) d.(dbody))
   | None => None
   end.
 
 Definition is_constructor n ts :=
   match List.nth_error ts n with
   | Some a =>
-    match a with
+    let (f, a) := decompose_app a in
+    match f with
     | tConstruct _ _ _ => true
-    | tApp (tConstruct _ _ _) _ => true
     | _ => false
     end
   | None => false
   end.
 
-Definition tDummy := tRel 0.
+Lemma fix_subst_length mfix : #|fix_subst mfix| = #|mfix|.
+Proof.
+  unfold fix_subst. generalize (tFix mfix). intros.
+  induction mfix; simpl; auto.
+Qed.
+
+Lemma cofix_subst_length mfix : #|cofix_subst mfix| = #|mfix|.
+Proof.
+  unfold cofix_subst. generalize (tCoFix mfix). intros.
+  induction mfix; simpl; auto.
+Qed.
+
+Definition fix_context (m : mfixpoint term) : context :=
+  List.rev (mapi (fun i d => vass d.(dname) (lift0 i d.(dtype))) m).
+
+Lemma fix_context_length mfix : #|fix_context mfix| = #|mfix|.
+Proof. unfold fix_context. now rewrite List.rev_length, mapi_length. Qed.
+
+Definition tDummy := tVar "".
 
 Definition iota_red npar c args brs :=
   (mkApps (snd (List.nth c brs (0, tDummy))) (List.skipn npar args)).
-
-Notation "#| Γ |" := (List.length Γ) (at level 0, Γ at level 99, format "#| Γ |").
