extraction/theories/WcbvEval.v
@@ -23,77 +23,30 @@ Existing Instance config.default_checker_flags.
   the extraction conjecture that can be applied to Coq terms to produce
   (untyped) terms where all proofs are erased to a dummy value. *)
 
-(** Helpers for reduction *)
-
-Definition iota_red npar c args brs :=
-  (mkApps (snd (List.nth c brs (0, tBox))) (List.skipn npar args)).
-
-Definition fix_subst (l : mfixpoint term) :=
-  let fix aux n :=
-      match n with
-      | 0 => []
-      | S n => tFix l n :: aux n
-      end
-  in aux (List.length l).
-
-Definition unfold_fix (mfix : mfixpoint term) (idx : nat) :=
-  match List.nth_error mfix idx with
-  | Some d => Some (d.(rarg), substl (fix_subst mfix) d.(dbody))
-  | None => None
-  end.
-
-Definition is_constructor n ts :=
-  match List.nth_error ts n with
-  | Some a =>
-    match a with
-    | tConstruct _ _ _ => true
-    | tApp (tConstruct _ _ _) _ => true
-    | _ => false
-    end
-  | None => false
-  end.
-
-
-Definition mktApp f l :=
-  match l with
-  | nil => f
-  | l => tApp f l
-  end.
-
 (** ** Big step version of weak cbv beta-zeta-iota-fix-delta reduction.
 
   TODO: CoFixpoints *)
 
 Section Wcbv.
-  Context (Σ : global_declarations) (Γ : context).
+  Context (Σ : global_declarations).
   (* The local context is fixed: we are only doing weak reductions *)
 
   Inductive eval : term -> term -> Prop :=
   (** Reductions *)
-  | eval_box l : eval (mktApp tBox l) tBox
+  | eval_box l : eval (mkApps tBox l) tBox
 
   (** Beta *)
-  | eval_beta f na t b a a' l res :
+  | eval_beta f na t b a a' res :
       eval f (tLambda na t b) ->
       eval a a' ->
-      eval (mkApps (subst0 a' b) l) res ->
-      eval (tApp f (a :: l)) res
+      eval (subst10 a' b) res ->
+      eval (tApp f a) res
 
   (** Let *)
   | eval_zeta na b0 b0' t b1 res :
       eval b0 b0' ->
-      eval (subst0 b0' b1) res ->
+      eval (subst10 b0' b1) res ->
       eval (tLetIn na b0 t b1) res
-
-  (** Local variables: defined or undefined *)
-  | eval_rel_def i (isdecl : i < List.length Γ) body res :
-      (safe_nth Γ (exist _ i isdecl)).(decl_body) = Some body ->
-      eval (lift0 (S i) body) res ->
-      eval (tRel i) res
-
-  | eval_rel_undef i (isdecl : i < List.length Γ) :
-      (safe_nth Γ (exist _ i isdecl)).(decl_body) = None ->
-      eval (tRel i) (tRel i)
 
   (** Case *)
   | eval_iota ind pars discr c u args p brs res :
@@ -104,10 +57,23 @@ Section Wcbv.
   (** Fix unfolding, with guard *)
   | eval_fix mfix idx args args' narg fn res :
       unfold_fix mfix idx = Some (narg, fn) ->
-      Forall2 eval args args' -> (* FIXME should we reduce the args after the recursive arg here? *)
-      is_constructor narg args' = true ->
+      Forall2 eval args args' -> (* QUESTION should we reduce the args after the recursive arg here? *)
+      is_constructor narg args' ->
       eval (mkApps fn args') res ->
       eval (mkApps (tFix mfix idx) args) res
+
+  (** CoFix-case unfolding *)
+  | red_cofix_case ip p mfix idx args narg fn brs res :
+      unfold_cofix mfix idx = Some (narg, fn) ->
+      eval (tCase ip (mkApps fn args) p brs) res ->
+      eval (tCase ip p (mkApps (tCoFix mfix idx) args) brs) res
+
+
+  (** CoFix-proj unfolding *)
+  | red_cofix_proj p mfix idx args narg fn res :
+      unfold_cofix mfix idx = Some (narg, fn) ->
+      eval (tProj p (mkApps fn args)) res ->
+      eval (tProj p (mkApps (tCoFix mfix idx) args)) res
 
   (** Constant unfolding *)
   | eval_delta c decl body (isdecl : declared_constant Σ c decl) u res :
@@ -121,26 +87,14 @@ Section Wcbv.
       eval (List.nth (pars + arg) args tDummy) res ->
       eval (tProj (i, pars, arg) discr) res
 
-  (* TODO CoFix *)
+  (** Abstractions are values *)
   | eval_abs na M N : eval (tLambda na M N) (tLambda na M N)
 
-  | eval_prod na b t b' t' :
-      eval b b' -> eval t t' -> eval (tProd na b t) (tProd na b' t')
-
-  | eval_ind_ i u : eval (tInd i u) (tInd i u)
-
-  | eval_app_ind t i u l l' : l <> nil ->
-      eval t (tInd i u) ->
-      Forall2 eval l l' ->
-      eval (tApp t l) (tApp (tInd i u) l')
-
-  | eval_constr i k u :
-      eval (tConstruct i k u) (tConstruct i k u)
-
-  | eval_app_constr f i k u l l' : l <> nil ->
+  (** Constructors applied to values are values *)
+  | eval_constr f i k u l l' :
       eval f (tConstruct i k u) ->
       Forall2 eval l l' ->
-      eval (tApp f l) (tApp (tConstruct i k u) l')
+      eval (mkApps f l) (mkApps (tConstruct i k u) l')
 
   (* | evar ev l l' : evals l l' -> eval (tEvar ev l) (tEvar ev l') *)
   | eval_evar ev l : eval (tEvar ev l) (tEvar ev l) (* Lets say it is a value for now *).
@@ -149,22 +103,16 @@ Section Wcbv.
 
   Lemma eval_evals_ind :
     forall P : term -> term -> Prop,
-      (forall l, P (mktApp tBox l) tBox) ->
-      (forall (f : term) (na : name) (t b a a' : term) (l : list term) (res : term),
+      (forall l, P (mkApps tBox l) tBox) ->
+      (forall (f : term) (na : name) (t b a a' : term) (res : term),
           eval f (tLambda na t b) ->
           P f (tLambda na t b) ->
           eval a a' -> P a a' ->
-          eval (mkApps (b {0 := a'}) l) res -> P (mkApps (b {0 := a'}) l) res -> P (tApp f (a :: l)) res) ->
+          eval (b {0 := a'}) res -> P (b {0 := a'}) res -> P (tApp f a) res) ->
 
       (forall (na : name) (b0 b0' t b1 res : term),
-          eval b0 b0' -> P b0 b0' -> eval (b1 {0 := b0'}) res -> P (b1 {0 := b0'}) res -> P (tLetIn na b0 t b1) res) ->
-
-      (forall (i : nat) (isdecl : i < #|Γ|) (body res : term),
-          decl_body (safe_nth Γ (exist (fun n : nat => n < #|Γ|) i isdecl)) = Some body ->
-          eval ((lift0 (S i)) body) res -> P ((lift0 (S i)) body) res -> P (tRel i) res) ->
-
-      (forall (i : nat) (isdecl : i < #|Γ|),
-          decl_body (safe_nth Γ (exist (fun n : nat => n < #|Γ|) i isdecl)) = None -> P (tRel i) (tRel i)) ->
+          eval b0 b0' -> P b0 b0' -> eval (b1 {0 := b0'}) res -> P (b1 {0 := b0'}) res ->
+          P (tLetIn na b0 t b1) res) ->
 
       (forall (ind : inductive) (pars : nat) (discr : term) (c : nat) (u : universe_instance)
               (args : list term) (p : term) (brs : list (nat * term)) (res : term),
@@ -179,6 +127,17 @@ Section Wcbv.
           Forall2 P args args' ->
           is_constructor narg args' = true ->
           eval (mkApps fn args') res -> P (mkApps fn args') res -> P (mkApps (tFix mfix idx) args) res) ->
+
+      (forall (ip : inductive * nat) (p : term) (mfix : mfixpoint term) (idx : nat) (args : list term)
+              (narg : nat) (fn : term) (brs : list (nat * term)) (res : term),
+          unfold_cofix mfix idx = Some (narg, fn) ->
+          eval (tCase ip (mkApps fn args) p brs) res ->
+          P (tCase ip (mkApps fn args) p brs) res -> P (tCase ip p (mkApps (tCoFix mfix idx) args) brs) res) ->
+
+      (forall (p : projection) (mfix : mfixpoint term) (idx : nat) (args : list term) (narg : nat) (fn res : term),
+          unfold_cofix mfix idx = Some (narg, fn) ->
+          eval (tProj p (mkApps fn args)) res ->
+          P (tProj p (mkApps fn args)) res -> P (tProj p (mkApps (tCoFix mfix idx) args)) res) ->
 
       (forall (c : ident) (decl : constant_body) (body : term),
           declared_constant Σ c decl ->
@@ -195,27 +154,16 @@ Section Wcbv.
 
       (forall (na : name) (M N : term), P (tLambda na M N) (tLambda na M N)) ->
 
-      (forall (na : name) (M M' N N' : term),
-          eval M M' -> eval N N' -> P M M' -> P N N' ->
-          P (tProd na M N) (tProd na M' N')) ->
-
-      (forall i u, P (tInd i u) (tInd i u)) ->
-
-      (forall (f8 : term) (i : inductive) (u : universe_instance) (l l' : list term),
-          l <> nil -> eval f8 (tInd i u) ->
-          P f8 (tInd i u) -> Forall2 eval l l' -> Forall2 P l l' -> P (tApp f8 l) (tApp (tInd i u) l')) ->
-
-      (forall i k u, P (tConstruct i k u) (tConstruct i k u)) ->
-
       (forall (f8 : term) (i : inductive) (k : nat) (u : universe_instance) (l l' : list term),
-          l <> nil -> eval f8 (tConstruct i k u) ->
-          P f8 (tConstruct i k u) -> Forall2 eval l l' -> Forall2 P l l' -> P (tApp f8 l) (tApp (tConstruct i k u) l')) ->
+          eval f8 (tConstruct i k u) ->
+          P f8 (tConstruct i k u) -> Forall2 eval l l' -> Forall2 P l l' -> P (mkApps f8 l) (mkApps (tConstruct i k u) l')) ->
 
       (forall (ev : nat) (l : list term), P (tEvar ev l) (tEvar ev l)) ->
 
       forall t t0 : term, eval t t0 -> P t t0.
   Proof.
-    intros P Hbox Hbeta Hlet Hreldef Hrelvar Hcase Hfix Hconst Hproj Hlam Hprod Hind Hindapp Hcstr Hcstrapp Hevar.
+    intros P Hbox Hbeta Hlet Hcase Hfix Hcoficase Hcofixproj
+           Hconst Hproj Hlam Hcstr Hevar.
     fix eval_evals_ind 3. destruct 1;
              try match goal with [ H : _ |- _ ] =>
                              match type of H with
@@ -225,12 +173,8 @@ Section Wcbv.
     clear H1 H2.
     revert args args' H0. fix aux 3. destruct 1. constructor; auto.
     constructor. now apply eval_evals_ind. now apply aux.
-    revert l l' H H1. fix aux 4. destruct 2. contradiction. constructor.
-    now apply eval_evals_ind.
-    destruct l. inv H2; constructor.
-    now apply aux.
-    revert l l' H H1. fix aux 4. destruct 2. contradiction. constructor.
-    now apply eval_evals_ind. destruct l. inv H2; constructor. now apply aux.
+    revert l l' H0. fix aux 3. destruct 1; constructor.
+    now apply eval_evals_ind. apply aux. auto.
   Defined.
 
   (** Characterization of values for this reduction relation:
@@ -240,11 +184,8 @@ Section Wcbv.
 
   Inductive value : term -> Prop :=
   | value_tBox : value tBox
-  | value_tRel i : value (tRel i)
   | value_tEvar ev l : value (tEvar ev l)
   | value_tLam na t b : value (tLambda na t b)
-  | value_tProd na t u : value (tProd na t u)
-  | value_tInd i k l : List.Forall value l -> value (mkApps (tInd i k) l)
   | value_tConstruct i k u l : List.Forall value l -> value (mkApps (tConstruct i k u) l).
 
   Lemma value_values_ind : forall P : term -> Prop,
@@ -252,47 +193,25 @@ Section Wcbv.
        (forall i : nat, P (tRel i)) ->
        (forall (ev : nat) (l : list term), P (tEvar ev l)) ->
        (forall (na : name) (t b : term), P (tLambda na t b)) ->
-       (forall (na : name) (t u : term), P (tProd na t u)) ->
-       (forall (i : inductive) (k : universe_instance) l, List.Forall value l -> List.Forall P l -> P (mkApps (tInd i k) l)) ->
        (forall (i : inductive) (k : nat) (u : universe_instance) (l : list term),
-        List.Forall value l -> List.Forall P l -> P (mkApps (tConstruct i k u) l)) -> forall t : term, value t -> P t.
+           List.Forall value l -> List.Forall P l -> P (mkApps (tConstruct i k u) l)) ->
+       forall t : term, value t -> P t.
   Proof.
-    intros P ???????.
-    fix value_values_ind 2. destruct 1. 1-4:clear value_values_ind; auto.
-    apply H3. apply H4. apply H6.
-    revert l H6. fix aux 2. destruct 1. constructor; auto.
-    constructor. now apply value_values_ind. now apply aux.
-    apply H5. apply H6.
-    revert l H6. fix aux 2. destruct 1. constructor; auto.
+    intros P ?????.
+    fix value_values_ind 2. destruct 1. 1-3:clear value_values_ind; auto.
+    apply H3. apply H4.
+    revert l H4. fix aux 2. destruct 1. constructor; auto.
     constructor. now apply value_values_ind. now apply aux.
   Defined.
 
   (** The codomain of evaluation is only values:
       It means no redex can remain at the head of an evaluated term. *)
 
-  Lemma Forall2_right {A B} (P : B -> Prop) (l : list A) (l' : list B) :
-    Forall2 (fun x y => P y) l l' -> List.Forall (fun x => P x) l'.
-  Proof.
-    induction 1; constructor; auto.
-  Qed.
-
-  Lemma Forall2_non_nil {A B} (P : A -> B -> Prop) (l : list A) (l' : list B) :
-    Forall2 P l l' -> l <> nil -> l' <> nil.
-  Proof.
-    induction 1; congruence.
-  Qed.
-
   Lemma eval_to_value e e' : eval e e' -> value e'.
   Proof.
     induction 1 using eval_evals_ind; simpl; auto using value.
-    eapply (value_tInd i u []); try constructor.
-    pose proof (value_tInd i u l'). forward H3.
-    apply (Forall2_right _ _ _ H2).
-    rewrite mkApps_tApp in H3; auto. simpl; auto. eauto using Forall2_non_nil.
-    eapply (value_tConstruct i k u []); try constructor.
-    pose proof (value_tConstruct i k u l'). forward H3.
-    apply (Forall2_right _ _ _ H2).
-    rewrite mkApps_tApp in H3; auto. simpl; auto. eauto using Forall2_non_nil.
+    eapply (value_tConstruct i k u).
+    apply (Forall2_right _ _ _ H1).
   Qed.
 
   (** Evaluation preserves closedness: *)
