extraction/theories/AstUtils.v
@@ -1,0 +1,16 @@
+From Coq Require Import Ascii String Bool OrderedType Lia List Program Arith.
+From Template Require Import utils Ast.
+From TemplateExtraction Require Import Ast.
+Import List.ListNotations.
+Require Import FunctionalExtensionality.
+Require Import ssreflect.
+
+Set Asymmetric Patterns.
+
+Fixpoint decompose_app_rec t l :=
+  match t with
+  | tApp f a => decompose_app_rec f (a :: l)
+  | f => (f, l)
+  end.
+
+Definition decompose_app f := decompose_app_rec f [].
