extraction/theories/Extraction.v
@@ -4,12 +4,6 @@
     should use these same directives for consistency.
 *)
 
-From TemplateExtraction Require Import Ast.
-From TemplateExtraction Require Import Induction.
-From TemplateExtraction Require Import LiftSubst.
-From TemplateExtraction Require Import UnivSubst.
-From TemplateExtraction Require Import Typing.
-
 Require Import FSets.
 Require Import ExtrOcamlBasic.
 Require Import ExtrOcamlString ExtrOcamlZInt.
@@ -18,14 +12,26 @@ Require Import ExtrOcamlString ExtrOcamlZInt.
    https://github.com/coq/coq/issues/7017. *)
 Extract Inductive Decimal.int => unit [ "(fun _ -> ())" "(fun _ -> ())" ] "(fun _ _ _ -> assert false)".
 
-Extraction Blacklist config uGraph univ Ast String List Nat UnivSubst UnivSubst0
+Extraction Blacklist config uGraph univ Ast AstUtils String List Nat UnivSubst UnivSubst0
            LiftSubst Induction Typing Retyping Typing0 Checker.
 Set Warnings "-extraction-opaque-accessed".
 
+From TemplateExtraction Require Import Ast.
 Extraction Library Ast.
+
+From TemplateExtraction Require Import AstUtils.
+Extraction Library AstUtils.
+
+From TemplateExtraction Require Import UnivSubst.
 Extraction Library UnivSubst.
+
+From TemplateExtraction Require Import Induction.
 Extraction Library Induction.
+
+From TemplateExtraction Require Import LiftSubst.
 Extraction Library LiftSubst.
+
+From TemplateExtraction Require Import Typing.
 Extraction Library Typing.
 
 (** Do it here, otherwise, LiftSubst, Typing etc refer to the ones of Template!
